src/EqbSpec.v
@@ -1,12 +1,18 @@
 From coqutil Require Import Option.
 
+Definition pair_eqb {A B} (eqbA : A -> A -> bool) (eqbB : B -> B -> bool)
+           (p1 p2 : A * B) : bool :=
+  let (a1, b1) := p1 in
+  let (a2, b2) := p2 in
+  eqbA a1 a2 && eqbB b1 b2.
+
 Lemma pair_eqb_spec {A B} (eqbA : A -> A -> bool) (eqbB : B -> B -> bool)
       (specA : forall x y, BoolSpec (x = y) (x <> y) (eqbA x y))
       (specB : forall x y, BoolSpec (x = y) (x <> y) (eqbB x y))
       (p1 p2 : A * B) :
-  BoolSpec (p1 = p2) (p1 <> p2)
-           (let (a1,b1) := p1 in let (a2,b2) := p2 in eqbA a1 a2 && eqbB b1 b2).
+  BoolSpec (p1 = p2) (p1 <> p2) (pair_eqb eqbA eqbB p1 p2).
 Proof.
+  unfold pair_eqb.
   destruct p1 as [a1 b1], p2 as [a2 b2].
   destruct (specA a1 a2); destruct (specB b1 b2); constructor; congruence.
 Qed.
