src/Examples/Layouts/GridLayout.v
@@ -1,27 +1,95 @@
-From Stdlib Require Import List.
-From DatalogRocq Require Import Dataflow GridGraph DependencyGenerator ATLDatalogParams Matmul.
-From Datalog Require Import CompilerExamples.
-From coqutil Require Import Map.Interface Map.Properties Map.Solver.
+From Stdlib Require Import List Bool Lia.
+From Datalog Require Import Datalog.
+From DatalogRocq Require Import Dataflow GridGraph DependencyGenerator.
 Import ListNotations.
 
-Definition three_three_dims : list nat := [3; 3].
+Module GridLayout (Params : DatalogParams).
+  Import Params.
+  Parameter (dims : list nat).
+  Definition rule := Datalog.rule rel var fn aggregator.
+  Parameter (program : list rule).
+  Parameter (indexed_layout : list (Node * list nat)).
+  Module dependency_generator := DependencyGenerator(Params).
 
-Definition three_three_grid_graph := GridGraph three_three_dims.
+  Definition grid_graph : Dataflow.Graph := GridGraph dims.
 
-Definition indexed_layout : list (Node * list nat) := [].
+  Definition layout (n : Node) : list rule :=
+    if check_node_in_bounds dims n then
+      match find (fun p => GridGraph.node_eqb (fst p) n) indexed_layout with
+      | None => []
+      | Some (_, ris) =>
+          fold_right
+            (fun ri acc =>
+               match nth_error program ri with
+               | Some r => r :: acc
+               | None => acc
+               end)
+            [] ris
+      end
+    else [].
 
-Definition layout (n : Node) : list rule := 
- match find (fun p => if GridGraph.node_eqb (fst p) n then true else false) indexed_layout with
-  | None => []
-  | Some (_, ris) =>
-      map (fun ri => nth ri datalog_matmul empty_rule) ris
-  end.
+  Definition rule_in_layout (r : rule) : bool :=
+    existsb (fun n => existsb (dependency_generator.rule_eqb r) (layout n))
+            (all_nodes_h dims).
+
+  Definition node_rules_ok (n : Node) : bool :=
+    forallb (fun r => existsb (dependency_generator.rule_eqb r) program)
+            (layout n).
+
+  Definition check_layout : bool :=
+    forallb node_rules_ok (all_nodes_h dims) &&
+    forallb rule_in_layout program.
+
+  Lemma layout_nonempty_only_valid_nodes :
+    forall n r,
+      In r (layout n) ->
+      GridGraph.is_graph_node dims n.
+  Proof.
+    intros n r Hlayout.
+    unfold layout in Hlayout.
+    destruct (check_node_in_bounds dims n) eqn:Hbounds; try discriminate.
+    - apply GridGraph.check_node_in_bounds_h_correct; eauto.
+    - contradiction.
+  Qed.
+
 
 Theorem good_layout :
-  Dataflow.good_layout layout three_three_grid_graph.(nodes) datalog_matmul.
+  check_layout = true ->
+  Dataflow.good_layout layout grid_graph.(nodes) program.
 Proof.
+    unfold check_layout.
     unfold Dataflow.good_layout.
+    intros.
     split.
-    - apply Forall_forall. intros. admit.
-    - intros. split.
-Admitted.
+    - apply Forall_forall. intros. apply andb_true_iff in H. destruct H as [H_nodes_ok H_rule_in_layout].
+      rewrite forallb_forall in H_rule_in_layout.
+      apply H_rule_in_layout in H0 as H_layout.
+      unfold rule_in_layout in H_layout. rewrite existsb_exists in H_layout.
+      destruct H_layout as [n [H_n_in_nodes H_r_in_layout]].
+      rewrite existsb_exists in H_r_in_layout.
+      destruct H_r_in_layout as [r H_r_eq].
+      exists n. destruct H_r_eq as [Hin H_r_eq]. 
+      destruct (dependency_generator.rule_eqb_spec x r).
+      + subst. split; auto. apply all_nodes_correct. apply H_n_in_nodes.
+      + discriminate H_r_eq.
+    - intros.
+      apply andb_true_iff in H. destruct H as [H_nodes_ok H_rule_in_layout].
+      rewrite forallb_forall in H_nodes_ok.
+      rewrite forallb_forall in H_rule_in_layout.
+      split.
+      + apply layout_nonempty_only_valid_nodes in H0 as H_layout_nonempty.
+        auto.
+      + apply layout_nonempty_only_valid_nodes in H0 as H_layout_nonempty.
+        apply all_nodes_correct in H_layout_nonempty.
+        specialize (H_nodes_ok n H_layout_nonempty).
+        unfold node_rules_ok in H_nodes_ok.
+        rewrite forallb_forall in H_nodes_ok.
+        specialize (H_nodes_ok r H0).
+        rewrite existsb_exists in H_nodes_ok.
+        destruct H_nodes_ok as [r' H_r'_in_program].
+        destruct H_r'_in_program as [Hin H_r_eq].
+        destruct (dependency_generator.rule_eqb_spec r r').
+        * subst. auto.
+        * discriminate H_r_eq.
+Qed.
+
